theories/typing/bitfield.v
@@ -265,7 +265,8 @@ Section programs.
 
   Lemma type_if_bitfield_raw it n v T1 T2:
     destruct_hint (DHintDecide (n ≠ 0)) (DestructHintIfInt n)
-      (if decide (n ≠ 0) then T1 else T2)
+      (li_trace (DestructHintIfInt n, if decide (n ≠ 0) then true else false)
+         (if decide (n ≠ 0) then T1 else T2))
     ⊢ typed_if (IntOp it) v (v ◁ᵥ n @ bitfield_raw it) T1 T2.
   Proof. unfold bitfield_raw; simpl_type. apply type_if_int. Qed.
   Definition type_if_bitfield_raw_inst := [instance type_if_bitfield_raw].
